src/Manifest_Generator_Facts_Static.v
@@ -1,5 +1,5 @@
 Require Import Maps Term_Defs_Core Manifest Eqb_Evidence
-Executable_Facts_Map
+Executable_Facts
   Manifest_Generator Executable_Defs_Prop.
 
 Require Import Auto.
@@ -9,17 +9,103 @@ Require Import StructTactics.
 Require Import List.
 Import ListNotations.
 
+Set Nested Proofs Allowed.
+
 
 Definition manifest_subset (m1:Manifest) (m2:Manifest) : Prop :=
   (forall i, In i (asps m1) -> In i (asps m2)) /\
   (forall p, In p (uuidPlcs m1) -> In p (uuidPlcs m2)) /\
   (forall q, In q (pubKeyPlcs m1) -> In q (pubKeyPlcs m2)).
 
+Check Maps.map_get.
+
 Definition Environment_subset (e1:EnvironmentM) (e2:EnvironmentM) : Prop := 
+  forall m1 p, 
+  Maps.map_get e1 p = Some m1 -> 
+
+  (exists m2, 
+    Maps.map_get e2 p = Some m2 /\
+    manifest_subset m1 m2
+  ).
+
+Lemma manifest_subset_refl : forall m,
+  manifest_subset m m.
+Proof.
+  intros.
+  unfold manifest_subset; intros.
+  split; intros; ff.
+Qed.
+
+Lemma env_subset_refl : forall e, 
+  Environment_subset e e.
+Proof.
+  intros.
+  unfold Environment_subset; intros.
+  exists m1.
+  split; ff.
   
+  apply manifest_subset_refl.
+Qed.
 
-Check manifest_generator'.
+  (*
+  Lemma env_subset_trans : forall e1 e2 e3,
+  Environment_subset e1 e2 ->
+  Environment_subset e2 e3 -> 
+  Environment_subset e1 e3.
+  Proof.
+  Admitted.
+  *)
 
+Lemma manifest_generator_cumul : forall t p e1 e2,
+    Environment_subset e1 e2 ->
+    Environment_subset e1 (manifest_generator' p t e2).
+  Proof.
+  Admitted.
+
+  Lemma exec_static_cumul : forall t p e1 e2,
+    executable_static t p e1 -> 
+    Environment_subset e1 e2 -> 
+    executable_static t p e2.
+  Proof.
+  Admitted.
+
+  Lemma fafafa : forall t p e1 e2,
+    Environment_subset e1 e2 ->
+    Environment_subset (manifest_generator' p t e1)
+                       (manifest_generator' p t e2).
+  Proof.
+    intros.
+    apply manifest_generator_cumul.
+
+    generalizeEverythingElse t.
+    induction t; intros; ff.
+    -
+    destruct a; ff;
+    unfold asp_manifest_generator; ff.
+    +
+      unfold Environment_subset in *; intros.
+      apply H.
+      Check eqb_plc.
+      destruct (eqb_plc p p0) eqn:hi.
+      ++
+      assert (m = m1). admit.
+      subst.
+      rewrite eqb_eq_plc in *.
+      subst.
+      eassumption.
+      ++
+      admit.
+    +
+      unfold Environment_subset in *; intros.
+      apply H.
+      destruct (eqb_plc p p0) eqn:hi.
+      ++
+      
+      rewrite eqb_eq_plc in *.
+      subst.
+      asdf.
+
+  Admitted.
 
 
 Theorem manifest_generator_executability_static :
@@ -72,13 +158,78 @@ Proof.
     +
     assert (executable_static t p (manifest_generator' p t e_empty)).
     { eauto. }
-    admit.
-    - (* lseq case *) 
-      admit.   
-    - (* bseq case *) 
-      admit.
-    - (* bpar case *) 
-    admit.    
+
+  eapply exec_static_cumul.
+  eassumption.
+
+  apply fafafa.
+
+  unfold Environment_subset; intros.
+  exists m1.
+  ff.
+
+
+  - (* lseq case *)
+    unfold manifest_generator in *.
+    ff.
+    split.
+    +
+
+    eapply exec_static_cumul.
+    apply IHt1.
+
+    apply manifest_generator_cumul.
+
+    apply env_subset_refl.
+
+    +
+
+    eapply exec_static_cumul.
+    apply IHt2.
+    apply fafafa.
+    apply manifest_generator_cumul.
+    apply env_subset_refl.
+
+
+    - (* bseq case *)
+    unfold manifest_generator in *.
+    ff.
+    split.
+    +
+
+    eapply exec_static_cumul.
+    apply IHt1.
+
+    apply manifest_generator_cumul.
+    apply env_subset_refl.
+
+    +
+
+    eapply exec_static_cumul.
+    apply IHt2.
+    apply fafafa.
+    apply manifest_generator_cumul.
+    apply env_subset_refl.
+
+    - (* bpar case *)
+    unfold manifest_generator in *.
+    ff.
+    split.
+    +
+
+    eapply exec_static_cumul.
+    apply IHt1.
+
+    apply manifest_generator_cumul.
+    apply env_subset_refl.
+
+    +
+
+    eapply exec_static_cumul.
+    apply IHt2.
+    apply fafafa.
+    apply manifest_generator_cumul.
+    apply env_subset_refl.  
 
 Abort.
 
